src/library/fun_info.h
@@ -10,46 +10,20 @@ Author: Leonardo de Moura
 namespace lean {
 /** \brief Function parameter information. */
 class param_info {
-    /* m_specialized is true if the result of fun_info has been specifialized
-       using this argument.
-       For example, consider the function
-
-             f : Pi (A : Type), A -> A
-
-       Now, suppse we request get_specialize fun_info for the application
-
-             f unit a
-
-       fun_info_manager returns two param_info objects:
-       1) m_specialized = true, m_is_dep = true
-       2) m_subsingleton = true, m_deps = {0}
-
-       Note that, in general, the second argument of f is not a subsingleton,
-       but it is in this particular case/specialization.
-
-       \remark This bit is only set if it is a dependent parameter (i.e., m_is_dep is true).
-
-       Moreover, we only set m_specialized IF another parameter
-       becomes a subsingleton or proposition. */
-    unsigned       m_specialized:1;
     unsigned       m_implicit:1;
     unsigned       m_inst_implicit:1;
     unsigned       m_prop:1;
-    unsigned       m_subsingleton:1;
     unsigned       m_has_fwd_deps:1; // true if rest depends on this parameter
     list<unsigned> m_back_deps;      // previous arguments it depends on
 public:
-    param_info(bool spec, bool imp, bool inst_imp, bool prop, bool sub, bool has_fwd_deps, list<unsigned> const & back_deps):
-        m_specialized(spec), m_implicit(imp), m_inst_implicit(inst_imp), m_prop(prop), m_subsingleton(sub),
+    param_info(bool imp, bool inst_imp, bool prop, bool has_fwd_deps, list<unsigned> const & back_deps):
+        m_implicit(imp), m_inst_implicit(inst_imp), m_prop(prop),
         m_has_fwd_deps(has_fwd_deps), m_back_deps(back_deps) {}
     list<unsigned> const & get_back_deps() const { return m_back_deps; }
-    bool specialized() const { return m_specialized; }
     bool is_implicit() const { return m_implicit; }
     bool is_inst_implicit() const { return m_inst_implicit; }
     bool is_prop() const { return m_prop; }
-    bool is_subsingleton() const { return m_subsingleton; }
     bool has_fwd_deps() const { return m_has_fwd_deps; }
-    void set_specialized() { m_specialized = true; }
 };
 
 /** \brief Function information produced by get_fun_info procedures. */
@@ -70,24 +44,61 @@ fun_info get_fun_info(type_context & ctx, expr const & fn);
 /** \brief Return information assuming the function has only nargs.
     \pre nargs <= get_fun_info(ctx, fn).get_arity() */
 fun_info get_fun_info(type_context & ctx, expr const & fn, unsigned nargs);
-/** \brief Return information for the function application.
-    This is more precise than \c get methods for dependent functions.
+
+/** \brief Subsingleton parameter information */
+class subsingleton_param_info {
+    /* m_specialized is true if the result of fun_info has been specifialized
+       using this argument.
+       For example, consider the function
+
+             f : Pi (A : Type), A -> A
+
+       Now, suppse we request get_specialize fun_info for the application
+
+             f unit a
+
+       fun_info_manager returns two param_info objects:
+       1) m_specialized = true
+       2) m_subsingleton = true
+
+       Note that, in general, the second argument of f is not a subsingleton,
+       but it is in this particular case/specialization.
+
+       \remark This bit is only set if it is a dependent parameter (i.e., m_is_dep is true).
+
+       Moreover, we only set m_specialized IF another parameter
+       becomes a subsingleton or proposition. */
+    unsigned short m_specialized;
+    unsigned short m_subsingleton;
+public:
+    subsingleton_param_info(bool spec, bool ss):
+        m_specialized(spec), m_subsingleton(ss) {}
+    bool specialized() const { return m_specialized; }
+    bool is_subsingleton() const { return m_subsingleton; }
+    void set_specialized() { m_specialized = true; }
+};
+
+typedef subsingleton_param_info ss_param_info;
+typedef list<ss_param_info>     ss_param_infos;
+
+list<ss_param_info> get_subsingleton_info(type_context & ctx, expr const & fn);
+list<ss_param_info> get_subsingleton_info(type_context & ctx, expr const & fn, unsigned nargs);
+/** \brief Return subsingleton parameter information for the function application.
+    This is more precise than \c get_subsingleton_info for dependent functions.
 
     Example: given (f : Pi (A : Type), A -> A), \c get_specialized_fun_info for
 
     f unit b
 
     returns a \c fun_info with two param_info
-    1) m_specialized = true, m_is_dep = true
-    2) m_subsingleton = true, m_deps = {0}
+    1) m_specialized = true
+    2) m_subsingleton = true
 
     The second argument is marked as subsingleton only because the resulting information
-    is taking into account the first argument.
-
-    \remark \c get and \c get_specialization return the same result for all but
-    is_prop and is_subsingleton. */
-fun_info get_specialized_fun_info(type_context & ctx, expr const & app);
+    is taking into account the first argument. */
+list<ss_param_info> get_specialized_subsingleton_info(type_context & ctx, expr const & app);
 unsigned get_specialization_prefix_size(type_context & ctx, expr const & fn, unsigned nargs);
+
 /** Clear thread local cache */
 void clear_fun_info_cache();
 
