src/library/tactic/fun_info_tactics.cpp
@@ -14,19 +14,17 @@ namespace lean {
 inline vm_obj bb(bool b) { return mk_vm_bool(b); }
 /*
   structure param_info :=
-  (specialized : bool)
   (is_implicit : bool)
   (is_inst_implicit : bool)
   (is_prop : bool)
-  (is_subsingleton : bool)
   (has_fwd_deps : bool)
   (back_deps : list nat) -- previous parameters it depends on
 */
 vm_obj to_obj(param_info const & info) {
-    vm_obj args[7] = { bb(info.specialized()), bb(info.is_implicit()), bb(info.is_inst_implicit()),
-                       bb(info.is_prop()), bb(info.is_subsingleton()), bb(info.has_fwd_deps()),
+    vm_obj args[5] = { bb(info.is_implicit()), bb(info.is_inst_implicit()),
+                       bb(info.is_prop()), bb(info.has_fwd_deps()),
                        to_obj(info.get_back_deps()) };
-    return mk_vm_constructor(0, 7, args);
+    return mk_vm_constructor(0, 5, args);
 }
 
 vm_obj to_obj(list<param_info> const & ls) {
@@ -42,10 +40,22 @@ vm_obj to_obj(fun_info const & info) {
     return mk_vm_constructor(0, to_obj(info.get_params_info()), to_obj(info.get_result_deps()));
 }
 
+vm_obj to_obj(ss_param_info const & info) {
+    return mk_vm_constructor(0, bb(info.specialized()), bb(info.is_subsingleton()));
+}
+
+vm_obj to_obj(list<ss_param_info> const & ls) {
+    return to_vm_list(ls, [&](ss_param_info const & p) { return to_obj(p); });
+}
+
 #define TRY   LEAN_TACTIC_TRY
 #define CATCH LEAN_TACTIC_CATCH(to_tactic_state(s))
 
 static vm_obj mk_result(fun_info const & info, vm_obj const & s) {
+    return mk_tactic_success(to_obj(info), to_tactic_state(s));
+}
+
+static vm_obj mk_result(list<ss_param_info> const & info, vm_obj const & s) {
     return mk_tactic_success(to_obj(info), to_tactic_state(s));
 }
 
@@ -63,10 +73,24 @@ vm_obj tactic_get_fun_info_n(vm_obj const & m, vm_obj const & fn, vm_obj const &
     CATCH;
 }
 
-vm_obj tactic_get_spec_fun_info(vm_obj const & m, vm_obj const & app, vm_obj const & s) {
+vm_obj tactic_get_subsingleton_info(vm_obj const & m, vm_obj const & fn, vm_obj const & s) {
     TRY;
     type_context ctx = mk_type_context_for(s, m);
-    return mk_result(get_specialized_fun_info(ctx, to_expr(app)), s);
+    return mk_result(get_subsingleton_info(ctx, to_expr(fn)), s);
+    CATCH;
+}
+
+vm_obj tactic_get_subsingleton_info_n(vm_obj const & m, vm_obj const & fn, vm_obj const & n, vm_obj const & s) {
+    TRY;
+    type_context ctx = mk_type_context_for(s, m);
+    return mk_result(get_subsingleton_info(ctx, to_expr(fn), force_to_unsigned(n, 0)), s);
+    CATCH;
+}
+
+vm_obj tactic_get_spec_subsingleton_info(vm_obj const & m, vm_obj const & app, vm_obj const & s) {
+    TRY;
+    type_context ctx = mk_type_context_for(s, m);
+    return mk_result(get_specialized_subsingleton_info(ctx, to_expr(app)), s);
     CATCH;
 }
 
@@ -79,10 +103,12 @@ vm_obj tactic_get_spec_prefix_size(vm_obj const & m, vm_obj const & fn, vm_obj c
 }
 
 void initialize_fun_info_tactics() {
-    DECLARE_VM_BUILTIN(name({"tactic", "get_fun_info_core"}),           tactic_get_fun_info);
-    DECLARE_VM_BUILTIN(name({"tactic", "get_fun_info_n_core"}),         tactic_get_fun_info_n);
-    DECLARE_VM_BUILTIN(name({"tactic", "get_spec_fun_info_core"}),      tactic_get_spec_fun_info);
-    DECLARE_VM_BUILTIN(name({"tactic", "get_spec_prefix_size_core"}),   tactic_get_spec_prefix_size);
+    DECLARE_VM_BUILTIN(name({"tactic", "get_fun_info_core"}),               tactic_get_fun_info);
+    DECLARE_VM_BUILTIN(name({"tactic", "get_fun_info_n_core"}),             tactic_get_fun_info_n);
+    DECLARE_VM_BUILTIN(name({"tactic", "get_subsingleton_info_core"}),      tactic_get_subsingleton_info);
+    DECLARE_VM_BUILTIN(name({"tactic", "get_subsingleton_info_n_core"}),    tactic_get_subsingleton_info_n);
+    DECLARE_VM_BUILTIN(name({"tactic", "get_spec_subsingleton_info_core"}), tactic_get_spec_subsingleton_info);
+    DECLARE_VM_BUILTIN(name({"tactic", "get_spec_prefix_size_core"}),       tactic_get_spec_prefix_size);
 }
 
 void finalize_fun_info_tactics() {
