library/init/meta/fun_info.lean
@@ -6,35 +6,10 @@ Authors: Leonardo de Moura
 prelude
 import init.meta.tactic init.meta.format init.function
 
-/- Function parameter information
-
-   Remark: specialized is tt if the result of fun_info has been specifialized
-   using this argument.
-   For example, consider the function
-
-            f : Pi (A : Type), A -> A
-
-   Now, suppse we request specialized_fun_info for the application
-
-             f unit a
-
-   the tactic returns two param_info values:
-   1) specialized = tt,     has_fwd_dep = tt
-   2) is_subsingleton = tt, back_deps = [0]
-
-   Note that, in general, the second argument of f is not a subsingleton,
-   but it is in this particular case/specialization.
-
-   This bit is only set if it is a dependent parameter (i.e., has_fwd_dep is tt).
-
-   Moreover, we only set specialized IF another parameter
-   becomes a subsingleton or proposition. -/
 structure param_info :=
-(specialized      : bool)
 (is_implicit      : bool)
 (is_inst_implicit : bool)
 (is_prop          : bool)
-(is_subsingleton  : bool)
 (has_fwd_deps     : bool)
 (back_deps        : list nat) -- previous parameters it depends on
 
@@ -51,13 +26,11 @@ else f₁ ++ "," ++ line ++ f₂
 local infix `+++`:65 := concat_fields
 
 meta_definition param_info.to_format : param_info → format
-| (param_info.mk s i ii p s d ds) :=
+| (param_info.mk i ii p d ds) :=
 group ∘ cbrace $
-  when s "specialized" +++
   when i  "implicit" +++
   when ii "inst_implicit" +++
   when p  "prop" +++
-  when s  "subsingleton" +++
   when d  "has_fwd_deps" +++
   when (to_bool (length ds > 0)) ("back_deps := " ++ to_fmt ds)
 
@@ -68,38 +41,75 @@ structure fun_info :=
 (params      : list param_info)
 (result_deps : list nat) -- parameters the result type depends on
 
-meta_definition fun_info.to_format : fun_info → format
+meta_definition fun_info_to_format : fun_info → format
 | (fun_info.mk ps ds) :=
 group ∘ dcbrace $
   ppfield "params" ps +++
   ppfield "result_deps" ds
 
-meta_definition fun_info.has_to_format [instance] : has_to_format fun_info :=
-has_to_format.mk fun_info.to_format
+meta_definition fun_info_has_to_format [instance] : has_to_format fun_info :=
+has_to_format.mk fun_info_to_format
+
+/-
+  specialized is true if the result of fun_info has been specifialized
+  using this argument.
+  For example, consider the function
+
+             f : Pi (A : Type), A -> A
+
+  Now, suppse we request get_specialize fun_info for the application
+
+         f unit a
+
+  fun_info_manager returns two param_info objects:
+  1) specialized = true
+  2) is_subsingleton = true
+
+  Note that, in general, the second argument of f is not a subsingleton,
+  but it is in this particular case/specialization.
+
+  \remark This bit is only set if it is a dependent parameter.
+
+   Moreover, we only set is_specialized IF another parameter
+   becomes a subsingleton -/
+structure subsingleton_info :=
+(specialized     : bool)
+(is_subsingleton : bool)
+
+meta_definition subsingleton_info_to_format : subsingleton_info → format
+| (subsingleton_info.mk s ss) :=
+group ∘ cbrace $
+  when s  "specialized" +++
+  when ss "subsingleton"
+
+meta_definition subsingleton_info_has_to_format [instance] : has_to_format subsingleton_info :=
+has_to_format.mk subsingleton_info_to_format
 
 namespace tactic
 meta_constant get_fun_info_core   : transparency → expr → tactic fun_info
 /- (get_fun_info fn n) return information assuming the function has only n arguments.
    The tactic fail if n > length (params (get_fun_info fn)) -/
 meta_constant get_fun_info_n_core : transparency → expr → nat → tactic fun_info
-/- (get_spec_func_info t) return information for the function application t of the form
-   (f a_1 ... a_n).
-   This tactic is more precise than (get_fun_info f) and (get_fun_info_n f)
 
-    Example: given (f : Pi (A : Type), A -> A), \c get_spec_func_info for
+meta_constant get_subsingleton_info_core : transparency → expr → tactic (list subsingleton_info)
+meta_constant get_subsingleton_info_n_core : transparency → expr → nat → tactic (list subsingleton_info)
+
+/- (get_spec_subsingleton_info t) return subsingleton parameter
+   information for the function application t of the form
+      (f a_1 ... a_n).
+   This tactic is more precise than (get_subsingleton_info f) and (get_subsingleton_info_n f n)
+
+    Example: given (f : Pi (A : Type), A -> A), \c get_spec_subsingleton_info for
 
     f unit b
 
     returns a fun_info with two param_info
-    1) specialized = tt, has_fwd_deps = tt
-    2) is_subsingleton = tt, back_deps = [0]
+    1) specialized = tt
+    2) is_subsingleton = tt
 
     The second argument is marked as subsingleton only because the resulting information
-    is taking into account the first argument.
-
-    Remark: get_fun_info and get_spec_func_info return the same result for all but
-    is_prop and is_subsingleton. -/
-meta_constant get_spec_fun_info_core   : transparency → expr → tactic fun_info
+    is taking into account the first argument. -/
+meta_constant get_spec_subsingleton_info_core : transparency → expr → tactic (list subsingleton_info)
 meta_constant get_spec_prefix_size_core : transparency → expr → nat → tactic nat
 
 meta_definition get_fun_info : expr → tactic fun_info :=
@@ -108,8 +118,14 @@ get_fun_info_core semireducible
 meta_definition get_fun_info_n : expr → nat → tactic fun_info :=
 get_fun_info_n_core semireducible
 
-meta_definition get_spec_fun_info : expr → tactic fun_info :=
-get_spec_fun_info_core semireducible
+meta_definition get_subsingleton_info : expr → tactic (list subsingleton_info) :=
+get_subsingleton_info_core semireducible
+
+meta_definition get_subsingleton_info_n : expr → nat → tactic (list subsingleton_info) :=
+get_subsingleton_info_n_core semireducible
+
+meta_definition get_spec_subsingleton_info : expr → tactic (list subsingleton_info) :=
+get_spec_subsingleton_info_core semireducible
 
 meta_definition get_spec_prefix_size : expr → nat → tactic nat :=
 get_spec_prefix_size_core semireducible
