library/init/default.lean
@@ -6,7 +6,7 @@ Authors: Leonardo de Moura
 prelude
 import init.datatypes init.reserved_notation init.logic
 import init.relation init.nat init.prod init.combinator
-import init.bool init.num init.sigma init.measurable init.setoid init.quot
+import init.bool init.unit init.num init.sigma init.measurable init.setoid init.quot
 import init.funext init.function init.subtype init.classical init.simplifier
 import init.monad init.option init.fin init.list init.char init.string init.to_string
 import init.timeit init.trace init.unsigned init.ordering init.list_classes
