library/init/unit.lean
@@ -1,0 +1,22 @@
+/-
+Copyright (c) 2016 Microsoft Corporation. All rights reserved.
+Released under Apache 2.0 license as described in the file LICENSE.
+Author: Leonardo de Moura
+-/
+prelude
+import init.logic
+
+theorem unit_eq (a b : unit) : a = b :=
+unit.rec_on a (unit.rec_on b rfl)
+
+theorem unit_eq_unit (a : unit) : a = () :=
+unit_eq a ()
+
+definition unit_subsingleton [instance] : subsingleton unit :=
+subsingleton.intro unit_eq
+
+definition unit_is_inhabited [instance] : inhabited unit :=
+inhabited.mk ()
+
+definition unit_has_decidable_eq [instance] : decidable_eq unit :=
+take (a b : unit), decidable.tt (unit_eq a b)
