tests/lean/run/fun_info1.lean
@@ -1,7 +1,14 @@
 open tactic
 
-example (a : nat) : true :=
+set_option pp.binder_types true
+definition foo (A : Type) : A → A :=
+sorry
+
+example (a : nat) (H : foo unit () = ()) : true :=
 by do
+  (lhs, rhs) ← get_local "H" >>= infer_type >>= match_eq ,
+  get_spec_subsingleton_info lhs >>= trace,
+  trace "-----------",
   trace "ite information:",
   mk_const "ite" >>= get_fun_info >>= trace,
   trace "eq.rec information:",
